prophecy/ProphecyHeader.v
@@ -1,4 +1,4 @@
-Require Import Common.
+Require Import Common Mod.
 Require Import Ensembles String.
 From stdpp Require Import base.
 
@@ -50,7 +50,20 @@ Module Prophecy.
 End Prophecy.
 
 Module ProphecyName.
-  Definition new := "Prophecy.new".
-  Definition resolve := "Prophecy.resolve".
-  Definition close := "Prophecy.close".
+  Definition new (mn : string) : string := "φ.new" ++ mn.
+  Definition resolve (mn : string) : string := "φ.resolve" ++ mn.
+  Definition close (mn : string) : string := "φ.close" ++ mn.
 End ProphecyName.
+
+Definition real_mod `{Σ : GRA} (md : Mod.t) : Prop :=
+  map_Forall
+    (λ _ (v : option (emask * fbody)),
+      match v with
+      | Some (msk, _) =>
+          (∀ P, msk _ (subevent _ (Assume P)) = false) ∧
+          ∀ X, msk _ (subevent _ (Take X)) = true → ∃ (P : Prop), X = P
+      | _ => False
+      end) (Mod.fnsems md).
+
+Definition exports mn : gset string :=
+    {[ ProphecyName.new mn; ProphecyName.resolve mn; ProphecyName.close mn ]}.
